squashed changes

src/Init/Data/Range/Polymorphic/Iterators.lean
@@ -14,107 +14,818 @@ public import Init.Data.Iterators.Combinators.Attach
 
 open Std.Iterators
 
-namespace Std.PRange
+namespace Std
+open PRange
+
+namespace Rcc
+
+variable {α : Type u}
 
 /--
 Internal function that constructs an iterator for a `PRange`. This is an internal function.
 Use `PRange.iter` instead, which requires importing `Std.Data.Iterators`.
 -/
 @[always_inline, inline]
-def Internal.iter {sl su α} [UpwardEnumerable α] [BoundedUpwardEnumerable sl α]
-    (r : PRange ⟨sl, su⟩ α) : Iter (α := RangeIterator su α) α :=
-  ⟨⟨BoundedUpwardEnumerable.init? r.lower, r.upper⟩⟩
+def Internal.iter [UpwardEnumerable α] (r : Rcc α) : Iter (α := Rxc.Iterator α) α :=
+  ⟨⟨some r.lower, r.upper⟩⟩
 
 /--
 Returns the elements of the given range as a list in ascending order, given that ranges of the given
 type and shape are finite and support this function.
 -/
 @[always_inline, inline, expose]
-def toList {sl su α} [UpwardEnumerable α] [BoundedUpwardEnumerable sl α]
-    [SupportsUpperBound su α]
-    (r : PRange ⟨sl, su⟩ α)
-    [Iterator (RangeIterator su α) Id α] [Finite (RangeIterator su α) Id]
-    [IteratorCollect (RangeIterator su α) Id Id] : List α :=
-  PRange.Internal.iter r |>.toList
+def toList [UpwardEnumerable α] (r : Rcc α)
+    [Iterator (Rxc.Iterator α) Id α] [Finite (Rxc.Iterator α) Id]
+    [IteratorCollect (Rxc.Iterator α) Id Id] : List α :=
+  Internal.iter r |>.toList
 
 /--
 Returns the elements of the given range as an array in ascending order, given that ranges of the
 given type and shape are finite and support this function.
 -/
 @[always_inline, inline, expose]
-def toArray {sl su α} [UpwardEnumerable α] [BoundedUpwardEnumerable sl α]
-    [SupportsUpperBound su α]
-    (r : PRange ⟨sl, su⟩ α)
-    [Iterator (RangeIterator su α) Id α] [Finite (RangeIterator su α) Id]
-    [IteratorCollect (RangeIterator su α) Id Id] : Array α :=
-  PRange.Internal.iter r |>.toArray
+def toArray {α} [UpwardEnumerable α] (r : Rcc α)
+    [Iterator (Rxc.Iterator α) Id α] [Finite (Rxc.Iterator α) Id]
+    [IteratorCollect (Rxc.Iterator α) Id Id] : Array α :=
+  Internal.iter r |>.toArray
 
 /--
 Iterators for ranges implementing `RangeSize` support the `size` function.
 -/
-instance [RangeSize su α] [UpwardEnumerable α] [SupportsUpperBound su α] :
-    IteratorSize (RangeIterator su α) Id where
+instance [Rxc.HasSize α] [UpwardEnumerable α] [LE α] [DecidableLE α] :
+    IteratorSize (Rxc.Iterator α) Id where
   size it := match it.internalState.next with
     | none => pure (.up 0)
-    | some next => pure (.up (RangeSize.size it.internalState.upperBound next))
+    | some next => pure (.up (Rxc.HasSize.size next it.internalState.upperBound))
 
 /--
 Returns the number of elements contained in the given range, given that ranges of the given
 type and shape support this function.
 -/
 @[always_inline, inline]
-def size {sl su α} [UpwardEnumerable α] [BoundedUpwardEnumerable sl α]
-    [SupportsUpperBound su α] (r : PRange ⟨sl, su⟩ α)
-    [IteratorSize (RangeIterator su α) Id] : Nat :=
-  PRange.Internal.iter r |>.size
+def size [UpwardEnumerable α] [LE α] [DecidableLE α] (r : Rcc α)
+    [IteratorSize (Rxc.Iterator α) Id] : Nat :=
+  Internal.iter r |>.size
 
 section Iterator
 
-theorem Internal.isPlausibleIndirectOutput_iter_iff {sl su α}
-    [UpwardEnumerable α] [BoundedUpwardEnumerable sl α]
-    [SupportsLowerBound sl α] [SupportsUpperBound su α]
-    [LawfulUpwardEnumerable α]
-    [LawfulUpwardEnumerableUpperBound su α] [LawfulUpwardEnumerableLowerBound sl α]
-    {r : PRange ⟨sl, su⟩ α} {a : α} :
-    (PRange.Internal.iter r).IsPlausibleIndirectOutput a ↔ a ∈ r := by
-  rw [RangeIterator.isPlausibleIndirectOutput_iff]
+theorem Internal.isPlausibleIndirectOutput_iter_iff
+    [UpwardEnumerable α] [LE α] [DecidableLE α]
+    [LawfulUpwardEnumerable α] [LawfulUpwardEnumerableLE α]
+    {r : Rcc α} {a : α} :
+    (Internal.iter r).IsPlausibleIndirectOutput a ↔ a ∈ r := by
+  rw [Rxc.Iterator.isPlausibleIndirectOutput_iff]
   constructor
   · rintro ⟨n, hn, hu⟩
     refine ⟨?_, hu⟩
-    rw [LawfulUpwardEnumerableLowerBound.isSatisfied_iff]
-    cases hr : (PRange.Internal.iter r).internalState.next
+    rw [LawfulUpwardEnumerableLE.le_iff]
+    cases hr : (Internal.iter r).internalState.next
     · simp [hr] at hn
     · rw [hr, Option.bind_some] at hn
-      exact ⟨_, hr, n, hn⟩
+      cases hr
+      exact ⟨n, hn⟩
   · rintro ⟨hl, hu⟩
-    rw [LawfulUpwardEnumerableLowerBound.isSatisfied_iff] at hl
-    obtain ⟨_, hr, n, hn⟩ := hl
-    exact ⟨n, by simp [PRange.Internal.iter, hr, hn], hu⟩
+    rw [LawfulUpwardEnumerableLE.le_iff] at hl
+    obtain ⟨n, hn⟩ := hl
+    exact ⟨n, by simp [Internal.iter, hn], hu⟩
 
-theorem RangeIterator.upwardEnumerableLe_of_isPlausibleIndirectOutput {su α}
-    [UpwardEnumerable α] [SupportsUpperBound su α]
-    [LawfulUpwardEnumerable α] [LawfulUpwardEnumerableUpperBound su α]
-    {it : Iter (α := RangeIterator su α) α} {out : α}
+open Std.Rxc.Iterator in
+theorem _root_.Std.Rxc.Iterator.upwardEnumerableLe_of_isPlausibleIndirectOutput
+    [UpwardEnumerable α] [LE α] [DecidableLE α]
+    [LawfulUpwardEnumerable α] [LawfulUpwardEnumerableLE α]
+    {it : Iter (α := Rxc.Iterator α) α} {out : α}
     (hout : it.IsPlausibleIndirectOutput out) :
     ∃ a, it.internalState.next = some a ∧ UpwardEnumerable.LE a out := by
-  have ⟨a, ha⟩ := Option.isSome_iff_exists.mp <|
-    RangeIterator.isSome_next_of_isPlausibleIndirectOutput hout
+  have ⟨a, ha⟩ := Option.isSome_iff_exists.mp (isSome_next_of_isPlausibleIndirectOutput hout)
   refine ⟨a, ha, ?_⟩
   simp only [isPlausibleIndirectOutput_iff, ha, Option.bind_some, exists_and_right] at hout
   exact hout.1
 
 @[no_expose]
-instance {sl su α m} [UpwardEnumerable α] [BoundedUpwardEnumerable sl α]
-    [SupportsLowerBound sl α] [SupportsUpperBound su α] [LawfulUpwardEnumerable α]
-    [LawfulUpwardEnumerableLowerBound sl α] [LawfulUpwardEnumerableUpperBound su α]
-    [Monad m] [Finite (RangeIterator su α) Id] :
-    ForIn' m (PRange ⟨sl, su⟩ α) α inferInstance where
+instance {m} [UpwardEnumerable α]
+    [LE α] [DecidableLE α] [LawfulUpwardEnumerable α] [LawfulUpwardEnumerableLE α]
+    [Monad m] [Finite (Rxc.Iterator α) Id] :
+    ForIn' m (Rcc α) α inferInstance where
   forIn' r init f := by
-    haveI := Iter.instForIn' (α := RangeIterator su α) (β := α) (n := m)
-    refine ForIn'.forIn' (α := α) (PRange.Internal.iter r) init (fun a ha acc => f a ?_ acc)
+    haveI := Iter.instForIn' (α := Rxc.Iterator α) (β := α) (n := m)
+    refine ForIn'.forIn' (α := α) (Internal.iter r) init (fun a ha acc => f a ?_ acc)
     simp only [Membership.mem] at ha
-    rwa [PRange.Internal.isPlausibleIndirectOutput_iter_iff] at ha
+    rwa [Internal.isPlausibleIndirectOutput_iter_iff] at ha
 
 end Iterator
 
-end Std.PRange
+end Rcc
+
+namespace Rco
+
+variable {α : Type u}
+
+/--
+Internal function that constructs an iterator for a `PRange`. This is an internal function.
+Use `PRange.iter` instead, which requires importing `Std.Data.Iterators`.
+-/
+@[always_inline, inline]
+def Internal.iter [UpwardEnumerable α] (r : Rco α) : Iter (α := Rxo.Iterator α) α :=
+  ⟨⟨some r.lower, r.upper⟩⟩
+
+/--
+Returns the elements of the given range as a list in ascending order, given that ranges of the given
+type and shape support this function and the range is finite.
+-/
+@[always_inline, inline, expose]
+def toList [UpwardEnumerable α] (r : Rco α)
+    [Iterator (Rxo.Iterator α) Id α] [Finite (Rxo.Iterator α) Id]
+    [IteratorCollect (Rxo.Iterator α) Id Id] : List α :=
+  Internal.iter r |>.toList
+
+/--
+Returns the elements of the given range as an array in ascending order, given that ranges of the
+given type and shape are finite and support this function.
+-/
+@[always_inline, inline, expose]
+def toArray {α} [UpwardEnumerable α] (r : Rco α)
+    [Iterator (Rxo.Iterator α) Id α] [Finite (Rxo.Iterator α) Id]
+    [IteratorCollect (Rxo.Iterator α) Id Id] : Array α :=
+  Internal.iter r |>.toArray
+
+/--
+Iterators for ranges implementing `RangeSize` support the `size` function.
+-/
+instance [Rxo.HasSize α] [UpwardEnumerable α] [LT α] [DecidableLT α] :
+    IteratorSize (Rxo.Iterator α) Id where
+  size it := match it.internalState.next with
+    | none => pure (.up 0)
+    | some next => pure (.up (Rxo.HasSize.size next it.internalState.upperBound))
+
+/--
+Returns the number of elements contained in the given range, given that ranges of the given
+type and shape support this function.
+-/
+@[always_inline, inline]
+def size [UpwardEnumerable α] [LT α] [DecidableLT α] (r : Rco α)
+    [IteratorSize (Rxo.Iterator α) Id] : Nat :=
+  Internal.iter r |>.size
+
+section Iterator
+
+theorem Internal.isPlausibleIndirectOutput_iter_iff
+    [UpwardEnumerable α] [LE α] [LT α] [DecidableLT α]
+    [LawfulUpwardEnumerable α] [LawfulUpwardEnumerableLT α] [LawfulUpwardEnumerableLE α]
+    {r : Rco α} {a : α} :
+    (Internal.iter r).IsPlausibleIndirectOutput a ↔ a ∈ r := by
+  rw [Rxo.Iterator.isPlausibleIndirectOutput_iff]
+  constructor
+  · rintro ⟨n, hn, hu⟩
+    refine ⟨?_, hu⟩
+    rw [LawfulUpwardEnumerableLE.le_iff]
+    cases hr : (Internal.iter r).internalState.next
+    · simp [hr] at hn
+    · rw [hr, Option.bind_some] at hn
+      cases hr
+      exact ⟨n, hn⟩
+  · rintro ⟨hl, hu⟩
+    rw [LawfulUpwardEnumerableLE.le_iff] at hl
+    obtain ⟨n, hn⟩ := hl
+    exact ⟨n, by simp [Internal.iter, hn], hu⟩
+
+open Std.Rxo.Iterator in
+theorem _root_.Std.Rxo.Iterator.upwardEnumerableLe_of_isPlausibleIndirectOutput
+    [UpwardEnumerable α] [LT α] [DecidableLT α]
+    [LawfulUpwardEnumerable α] [LawfulUpwardEnumerableLT α]
+    {it : Iter (α := Rxo.Iterator α) α} {out : α}
+    (hout : it.IsPlausibleIndirectOutput out) :
+    ∃ a, it.internalState.next = some a ∧ UpwardEnumerable.LE a out := by
+  have ⟨a, ha⟩ := Option.isSome_iff_exists.mp (isSome_next_of_isPlausibleIndirectOutput hout)
+  refine ⟨a, ha, ?_⟩
+  simp only [isPlausibleIndirectOutput_iff, ha, Option.bind_some, exists_and_right] at hout
+  exact hout.1
+
+@[no_expose]
+instance {m} [UpwardEnumerable α] [LE α] [LT α] [DecidableLT α]
+    [LawfulUpwardEnumerable α] [LawfulUpwardEnumerableLE α] [LawfulUpwardEnumerableLT α]
+    [Monad m] [Finite (Rxo.Iterator α) Id] :
+    ForIn' m (Rco α) α inferInstance where
+  forIn' r init f := by
+    haveI := Iter.instForIn' (α := Rxo.Iterator α) (β := α) (n := m)
+    refine ForIn'.forIn' (α := α) (Internal.iter r) init (fun a ha acc => f a ?_ acc)
+    simp only [Membership.mem] at ha
+    rwa [Internal.isPlausibleIndirectOutput_iter_iff] at ha
+
+end Iterator
+
+end Rco
+
+namespace Rci
+
+variable {α : Type u}
+
+/--
+Internal function that constructs an iterator for a `PRange`. This is an internal function.
+Use `PRange.iter` instead, which requires importing `Std.Data.Iterators`.
+-/
+@[always_inline, inline]
+def Internal.iter [UpwardEnumerable α] (r : Rci α) : Iter (α := Rxi.Iterator α) α :=
+  ⟨⟨some r.lower⟩⟩
+
+/--
+Returns the elements of the given range as a list in ascending order, given that ranges of the given
+type and shape support this function and the range is finite.
+-/
+@[always_inline, inline, expose]
+def toList [UpwardEnumerable α] (r : Rci α)
+    [Iterator (Rxi.Iterator α) Id α] [Finite (Rxi.Iterator α) Id]
+    [IteratorCollect (Rxi.Iterator α) Id Id] : List α :=
+  Internal.iter r |>.toList
+
+/--
+Returns the elements of the given range as an array in ascending order, given that ranges of the
+given type and shape are finite and support this function.
+-/
+@[always_inline, inline, expose]
+def toArray {α} [UpwardEnumerable α] (r : Rci α)
+    [Iterator (Rxi.Iterator α) Id α] [Finite (Rxi.Iterator α) Id]
+    [IteratorCollect (Rxi.Iterator α) Id Id] : Array α :=
+  Internal.iter r |>.toArray
+
+/--
+Iterators for ranges implementing `RangeSize` support the `size` function.
+-/
+instance [Rxi.HasSize α] [UpwardEnumerable α] :
+    IteratorSize (Rxi.Iterator α) Id where
+  size it := match it.internalState.next with
+    | none => pure (.up 0)
+    | some next => pure (.up (Rxi.HasSize.size next))
+
+/--
+Returns the number of elements contained in the given range, given that ranges of the given
+type and shape support this function.
+-/
+@[always_inline, inline]
+def size [UpwardEnumerable α] (r : Rci α)
+    [IteratorSize (Rxi.Iterator α) Id] : Nat :=
+  Internal.iter r |>.size
+
+section Iterator
+
+theorem Internal.isPlausibleIndirectOutput_iter_iff
+    [UpwardEnumerable α] [LE α] [LawfulUpwardEnumerable α]
+    [LawfulUpwardEnumerableLE α] {r : Rci α} {a : α} :
+    (Internal.iter r).IsPlausibleIndirectOutput a ↔ a ∈ r := by
+  rw [Rxi.Iterator.isPlausibleIndirectOutput_iff]
+  constructor
+  · rintro ⟨n, hn⟩
+    simp only [Membership.mem, LawfulUpwardEnumerableLE.le_iff]
+    cases hr : (Internal.iter r).internalState.next
+    · simp [hr] at hn
+    · rw [hr, Option.bind_some] at hn
+      cases hr
+      exact ⟨n, hn⟩
+  · intro hl
+    simp only [Membership.mem, LawfulUpwardEnumerableLE.le_iff] at hl
+    obtain ⟨n, hn⟩ := hl
+    exact ⟨n, by simp [Internal.iter, hn]⟩
+
+open Std.Rxi.Iterator in
+theorem _root_.Std.Rxi.Iterator.upwardEnumerableLe_of_isPlausibleIndirectOutput
+    [UpwardEnumerable α]
+    [LawfulUpwardEnumerable α]
+    {it : Iter (α := Rxi.Iterator α) α} {out : α}
+    (hout : it.IsPlausibleIndirectOutput out) :
+    ∃ a, it.internalState.next = some a ∧ UpwardEnumerable.LE a out := by
+  have ⟨a, ha⟩ := Option.isSome_iff_exists.mp (isSome_next_of_isPlausibleIndirectOutput hout)
+  refine ⟨a, ha, ?_⟩
+  simpa only [isPlausibleIndirectOutput_iff, ha, Option.bind_some] using hout
+
+@[no_expose]
+instance {m} [UpwardEnumerable α]
+    [LE α]
+    [LawfulUpwardEnumerable α] [LawfulUpwardEnumerableLE α]
+    [Monad m] [Finite (Rxi.Iterator α) Id] :
+    ForIn' m (Rci α) α inferInstance where
+  forIn' r init f := by
+    haveI := Iter.instForIn' (α := Rxi.Iterator α) (β := α) (n := m)
+    refine ForIn'.forIn' (α := α) (Internal.iter r) init (fun a ha acc => f a ?_ acc)
+    simp only [Membership.mem] at ha
+    rwa [Internal.isPlausibleIndirectOutput_iter_iff] at ha
+
+end Iterator
+
+end Rci
+
+namespace Roc
+
+variable {α : Type u}
+
+/--
+Internal function that constructs an iterator for a `PRange`. This is an internal function.
+Use `PRange.iter` instead, which requires importing `Std.Data.Iterators`.
+-/
+@[always_inline, inline]
+def Internal.iter [UpwardEnumerable α] (r : Roc α) : Iter (α := Rxc.Iterator α) α :=
+  ⟨⟨UpwardEnumerable.succ? r.lower, r.upper⟩⟩
+
+/--
+Returns the elements of the given range as a list in ascending order, given that ranges of the given
+type and shape support this function and the range is finite.
+-/
+@[always_inline, inline, expose]
+def toList [UpwardEnumerable α] (r : Roc α)
+    [Iterator (Rxc.Iterator α) Id α] [Finite (Rxc.Iterator α) Id]
+    [IteratorCollect (Rxc.Iterator α) Id Id] : List α :=
+  Internal.iter r |>.toList
+
+/--
+Returns the elements of the given range as an array in ascending order, given that ranges of the
+given type and shape are finite and support this function.
+-/
+@[always_inline, inline, expose]
+def toArray {α} [UpwardEnumerable α] (r : Roc α)
+    [Iterator (Rxc.Iterator α) Id α] [Finite (Rxc.Iterator α) Id]
+    [IteratorCollect (Rxc.Iterator α) Id Id] : Array α :=
+  Internal.iter r |>.toArray
+
+/--
+Iterators for ranges implementing `RangeSize` support the `size` function.
+-/
+instance [Rxc.HasSize α] [UpwardEnumerable α] [LE α] [DecidableLE α] :
+    IteratorSize (Rxc.Iterator α) Id where
+  size it := match it.internalState.next with
+    | none => pure (.up 0)
+    | some next => pure (.up (Rxc.HasSize.size next it.internalState.upperBound))
+
+/--
+Returns the number of elements contained in the given range, given that ranges of the given
+type and shape support this function.
+-/
+@[always_inline, inline]
+def size [UpwardEnumerable α] [LE α] [DecidableLE α] (r : Roc α)
+    [IteratorSize (Rxc.Iterator α) Id] : Nat :=
+  Internal.iter r |>.size
+
+section Iterator
+
+theorem Internal.isPlausibleIndirectOutput_iter_iff
+    [UpwardEnumerable α] [LE α] [DecidableLE α] [LT α]
+    [LawfulUpwardEnumerable α] [LawfulUpwardEnumerableLE α]
+    [LawfulUpwardEnumerableLT α]
+    {r : Roc α} {a : α} :
+    (Internal.iter r).IsPlausibleIndirectOutput a ↔ a ∈ r := by
+  rw [Rxc.Iterator.isPlausibleIndirectOutput_iff]
+  constructor
+  · rintro ⟨n, hn, hu⟩
+    refine ⟨?_, hu⟩
+    rw [LawfulUpwardEnumerableLT.lt_iff]
+    cases hr : (Internal.iter r).internalState.next
+    · simp [hr] at hn
+    · rw [hr, Option.bind_some] at hn
+      simp only [iter] at hr
+      apply UpwardEnumerable.lt_of_lt_of_le
+      · exact ⟨0, by simpa [UpwardEnumerable.succMany?_one]⟩
+      · exact ⟨_, hn⟩
+  · rintro ⟨hl, hu⟩
+    rw [LawfulUpwardEnumerableLT.lt_iff] at hl
+    obtain ⟨n, hn⟩ := hl
+    exact ⟨n,
+      by simp [Internal.iter, hn, ← UpwardEnumerable.succMany?_succ?_eq_succ?_bind_succMany?], hu⟩
+
+@[no_expose]
+instance {m} [UpwardEnumerable α]
+    [LE α] [DecidableLE α] [LawfulUpwardEnumerable α] [LawfulUpwardEnumerableLE α]
+    [LT α] [LawfulUpwardEnumerableLT α]
+    [Monad m] [Finite (Rxc.Iterator α) Id] :
+    ForIn' m (Roc α) α inferInstance where
+  forIn' r init f := by
+    haveI := Iter.instForIn' (α := Rxc.Iterator α) (β := α) (n := m)
+    refine ForIn'.forIn' (α := α) (Internal.iter r) init (fun a ha acc => f a ?_ acc)
+    simp only [Membership.mem] at ha
+    rwa [Internal.isPlausibleIndirectOutput_iter_iff] at ha
+
+end Iterator
+
+end Roc
+
+namespace Roo
+
+variable {α : Type u}
+
+/--
+Internal function that constructs an iterator for a `PRange`. This is an internal function.
+Use `PRange.iter` instead, which requires importing `Std.Data.Iterators`.
+-/
+@[always_inline, inline]
+def Internal.iter [UpwardEnumerable α] (r : Roo α) : Iter (α := Rxo.Iterator α) α :=
+  ⟨⟨UpwardEnumerable.succ? r.lower, r.upper⟩⟩
+
+/--
+Returns the elements of the given range as a list in ascending order, given that ranges of the given
+type and shape support this function and the range is finite.
+-/
+@[always_inline, inline, expose]
+def toList [UpwardEnumerable α] (r : Roo α)
+    [Iterator (Rxo.Iterator α) Id α] [Finite (Rxo.Iterator α) Id]
+    [IteratorCollect (Rxo.Iterator α) Id Id] : List α :=
+  Internal.iter r |>.toList
+
+/--
+Returns the elements of the given range as an array in ascending order, given that ranges of the
+given type and shape are finite and support this function.
+-/
+@[always_inline, inline, expose]
+def toArray {α} [UpwardEnumerable α] (r : Roo α)
+    [Iterator (Rxo.Iterator α) Id α] [Finite (Rxo.Iterator α) Id]
+    [IteratorCollect (Rxo.Iterator α) Id Id] : Array α :=
+  Internal.iter r |>.toArray
+
+/--
+Iterators for ranges implementing `RangeSize` support the `size` function.
+-/
+instance [Rxo.HasSize α] [UpwardEnumerable α] [LT α] [DecidableLT α] :
+    IteratorSize (Rxo.Iterator α) Id where
+  size it := match it.internalState.next with
+    | none => pure (.up 0)
+    | some next => pure (.up (Rxo.HasSize.size next it.internalState.upperBound))
+
+/--
+Returns the number of elements contained in the given range, given that ranges of the given
+type and shape support this function.
+-/
+@[always_inline, inline]
+def size [UpwardEnumerable α] [LT α] [DecidableLT α] (r : Roo α)
+    [IteratorSize (Rxo.Iterator α) Id] : Nat :=
+  Internal.iter r |>.size
+
+section Iterator
+
+theorem Internal.isPlausibleIndirectOutput_iter_iff
+    [UpwardEnumerable α] [LT α] [DecidableLT α] [LT α] [DecidableLT α]
+    [LawfulUpwardEnumerable α] [LawfulUpwardEnumerableLT α] [LawfulUpwardEnumerableLT α]
+    {r : Roo α} {a : α} :
+    (Internal.iter r).IsPlausibleIndirectOutput a ↔ a ∈ r := by
+  rw [Rxo.Iterator.isPlausibleIndirectOutput_iff]
+  constructor
+  · rintro ⟨n, hn, hu⟩
+    refine ⟨?_, hu⟩
+    rw [LawfulUpwardEnumerableLT.lt_iff]
+    cases hr : (Internal.iter r).internalState.next
+    · simp [hr] at hn
+    · rw [hr, Option.bind_some] at hn
+      simp only [iter] at hr
+      apply UpwardEnumerable.lt_of_lt_of_le
+      · exact ⟨0, by simpa [UpwardEnumerable.succMany?_one]⟩
+      · exact ⟨_, hn⟩
+  · rintro ⟨hl, hu⟩
+    rw [LawfulUpwardEnumerableLT.lt_iff] at hl
+    obtain ⟨n, hn⟩ := hl
+    exact ⟨n,
+      by simp [Internal.iter, hn, ← UpwardEnumerable.succMany?_succ?_eq_succ?_bind_succMany?], hu⟩
+
+@[no_expose]
+instance {m} [UpwardEnumerable α]
+    [LT α] [DecidableLT α]
+    [LawfulUpwardEnumerable α] [LawfulUpwardEnumerableLT α]
+    [Monad m] [Finite (Rxo.Iterator α) Id] :
+    ForIn' m (Roo α) α inferInstance where
+  forIn' r init f := by
+    haveI := Iter.instForIn' (α := Rxo.Iterator α) (β := α) (n := m)
+    refine ForIn'.forIn' (α := α) (Internal.iter r) init (fun a ha acc => f a ?_ acc)
+    simp only [Membership.mem] at ha
+    rwa [Internal.isPlausibleIndirectOutput_iter_iff] at ha
+
+end Iterator
+
+end Roo
+
+namespace Roi
+
+variable {α : Type u}
+
+/--
+Internal function that constructs an iterator for a `PRange`. This is an internal function.
+Use `PRange.iter` instead, which requires importing `Std.Data.Iterators`.
+-/
+@[always_inline, inline]
+def Internal.iter [UpwardEnumerable α] (r : Roi α) : Iter (α := Rxi.Iterator α) α :=
+  ⟨⟨UpwardEnumerable.succ? r.lower⟩⟩
+
+/--
+Returns the elements of the given range as a list in ascending order, given that ranges of the given
+type and shape support this function and the range is finite.
+-/
+@[always_inline, inline, expose]
+def toList [UpwardEnumerable α] (r : Roi α)
+    [Iterator (Rxi.Iterator α) Id α] [Finite (Rxi.Iterator α) Id]
+    [IteratorCollect (Rxi.Iterator α) Id Id] : List α :=
+  Internal.iter r |>.toList
+
+/--
+Returns the elements of the given range as an array in ascending order, given that ranges of the
+given type and shape are finite and support this function.
+-/
+@[always_inline, inline, expose]
+def toArray {α} [UpwardEnumerable α] (r : Roi α)
+    [Iterator (Rxi.Iterator α) Id α] [Finite (Rxi.Iterator α) Id]
+    [IteratorCollect (Rxi.Iterator α) Id Id] : Array α :=
+  Internal.iter r |>.toArray
+
+/--
+Iterators for ranges implementing `RangeSize` support the `size` function.
+-/
+instance [Rxi.HasSize α] [UpwardEnumerable α] :
+    IteratorSize (Rxi.Iterator α) Id where
+  size it := match it.internalState.next with
+    | none => pure (.up 0)
+    | some next => pure (.up (Rxi.HasSize.size next))
+
+/--
+Returns the number of elements contained in the given range, given that ranges of the given
+type and shape support this function.
+-/
+@[always_inline, inline]
+def size [UpwardEnumerable α] (r : Roi α)
+    [IteratorSize (Rxi.Iterator α) Id] : Nat :=
+  Internal.iter r |>.size
+
+section Iterator
+
+theorem Internal.isPlausibleIndirectOutput_iter_iff
+    [UpwardEnumerable α] [LT α] [LawfulUpwardEnumerable α]
+    [LawfulUpwardEnumerableLT α] {r : Roi α} {a : α} :
+    (Internal.iter r).IsPlausibleIndirectOutput a ↔ a ∈ r := by
+  rw [Rxi.Iterator.isPlausibleIndirectOutput_iff]
+  constructor
+  · rintro ⟨n, hn⟩
+    simp only [Membership.mem, LawfulUpwardEnumerableLT.lt_iff]
+    cases hr : (Internal.iter r).internalState.next
+    · simp [hr] at hn
+    · rw [hr, Option.bind_some] at hn
+      apply UpwardEnumerable.lt_of_lt_of_le
+      · exact ⟨0, by simpa [UpwardEnumerable.succMany?_one]⟩
+      · exact ⟨_, hn⟩
+  · intro hl
+    simp only [Membership.mem, LawfulUpwardEnumerableLT.lt_iff] at hl
+    obtain ⟨n, hn⟩ := hl
+    exact ⟨n,
+      by simp [Internal.iter, hn, ← UpwardEnumerable.succMany?_succ?_eq_succ?_bind_succMany?]⟩
+
+@[no_expose]
+instance {m} [UpwardEnumerable α]
+    [LT α] [LawfulUpwardEnumerable α] [LawfulUpwardEnumerableLT α]
+    [Monad m] [Finite (Rxi.Iterator α) Id] :
+    ForIn' m (Roi α) α inferInstance where
+  forIn' r init f := by
+    haveI := Iter.instForIn' (α := Rxi.Iterator α) (β := α) (n := m)
+    refine ForIn'.forIn' (α := α) (Internal.iter r) init (fun a ha acc => f a ?_ acc)
+    simp only [Membership.mem] at ha
+    rwa [Internal.isPlausibleIndirectOutput_iter_iff] at ha
+
+end Iterator
+
+end Roi
+
+namespace Ric
+
+variable {α : Type u}
+
+/--
+Internal function that constructs an iterator for a `PRange`. This is an internal function.
+Use `PRange.iter` instead, which requires importing `Std.Data.Iterators`.
+-/
+@[always_inline, inline]
+def Internal.iter [UpwardEnumerable α] [Least? α] (r : Ric α) : Iter (α := Rxc.Iterator α) α :=
+  ⟨⟨Least?.least?, r.upper⟩⟩
+
+/--
+Returns the elements of the given range as a list in ascending order, given that ranges of the given
+type and shape support this function and the range is finite.
+-/
+@[always_inline, inline, expose]
+def toList [UpwardEnumerable α] [Least? α] (r : Ric α)
+    [Iterator (Rxc.Iterator α) Id α] [Finite (Rxc.Iterator α) Id]
+    [IteratorCollect (Rxc.Iterator α) Id Id] : List α :=
+  Internal.iter r |>.toList
+
+/--
+Returns the elements of the given range as an array in ascending order, given that ranges of the
+given type and shape are finite and support this function.
+-/
+@[always_inline, inline, expose]
+def toArray {α} [UpwardEnumerable α] [Least? α] (r : Ric α)
+    [Iterator (Rxc.Iterator α) Id α] [Finite (Rxc.Iterator α) Id]
+    [IteratorCollect (Rxc.Iterator α) Id Id] : Array α :=
+  Internal.iter r |>.toArray
+
+/--
+Iterators for ranges implementing `RangeSize` support the `size` function.
+-/
+instance [Rxc.HasSize α] [UpwardEnumerable α] [LE α] [DecidableLE α] :
+    IteratorSize (Rxc.Iterator α) Id where
+  size it := match it.internalState.next with
+    | none => pure (.up 0)
+    | some next => pure (.up (Rxc.HasSize.size next it.internalState.upperBound))
+
+/--
+Returns the number of elements contained in the given range, given that ranges of the given
+type and shape support this function.
+-/
+@[always_inline, inline]
+def size [UpwardEnumerable α] [Least? α] [LE α] [DecidableLE α] (r : Ric α)
+    [IteratorSize (Rxc.Iterator α) Id] : Nat :=
+  Internal.iter r |>.size
+
+section Iterator
+
+theorem Internal.isPlausibleIndirectOutput_iter_iff
+    [UpwardEnumerable α] [Least? α] [LE α] [DecidableLE α]
+    [LawfulUpwardEnumerable α] [LawfulUpwardEnumerableLE α]
+    [LawfulUpwardEnumerableLeast? α]
+    {r : Ric α} {a : α} :
+    (Internal.iter r).IsPlausibleIndirectOutput a ↔ a ∈ r := by
+  rw [Rxc.Iterator.isPlausibleIndirectOutput_iff]
+  constructor
+  · rintro ⟨n, hn, hu⟩
+    simp only [Membership.mem, LawfulUpwardEnumerableLE.le_iff]
+    cases hr : (Internal.iter r).internalState.next
+    · simp [hr] at hn
+    · simpa [LawfulUpwardEnumerableLE.le_iff] using hu
+  · intro hu
+    obtain ⟨init, hi, hia⟩ := LawfulUpwardEnumerableLeast?.least?_le a
+    simpa [iter, hi] using ⟨hia, hu⟩
+
+@[no_expose]
+instance {m} [UpwardEnumerable α]
+    [LE α] [DecidableLE α] [Least? α]
+    [LawfulUpwardEnumerable α] [LawfulUpwardEnumerableLE α]
+    [LawfulUpwardEnumerableLeast? α]
+    [Monad m] [Finite (Rxc.Iterator α) Id] :
+    ForIn' m (Ric α) α inferInstance where
+  forIn' r init f := by
+    haveI := Iter.instForIn' (α := Rxc.Iterator α) (β := α) (n := m)
+    refine ForIn'.forIn' (α := α) (Internal.iter r) init (fun a ha acc => f a ?_ acc)
+    simp only [Membership.mem] at ha
+    rwa [Internal.isPlausibleIndirectOutput_iter_iff] at ha
+
+end Iterator
+
+end Ric
+
+namespace Rio
+
+variable {α : Type u}
+
+/--
+Internal function that constructs an iterator for a `PRange`. This is an internal function.
+Use `PRange.iter` instead, which requires importing `Std.Data.Iterators`.
+-/
+@[always_inline, inline]
+def Internal.iter [UpwardEnumerable α] [Least? α] (r : Rio α) : Iter (α := Rxo.Iterator α) α :=
+  ⟨⟨Least?.least?, r.upper⟩⟩
+
+/--
+Returns the elements of the given range as a list in ascending order, given that ranges of the given
+type and shape support this function and the range is finite.
+-/
+@[always_inline, inline, expose]
+def toList [UpwardEnumerable α] (r : Rio α) [Least? α]
+    [Iterator (Rxo.Iterator α) Id α] [Finite (Rxo.Iterator α) Id]
+    [IteratorCollect (Rxo.Iterator α) Id Id] : List α :=
+  Internal.iter r |>.toList
+
+/--
+Returns the elements of the given range as an array in ascending order, given that ranges of the
+given type and shape are finite and support this function.
+-/
+@[always_inline, inline, expose]
+def toArray {α} [UpwardEnumerable α] [Least? α] (r : Rio α)
+    [Iterator (Rxo.Iterator α) Id α] [Finite (Rxo.Iterator α) Id]
+    [IteratorCollect (Rxo.Iterator α) Id Id] : Array α :=
+  Internal.iter r |>.toArray
+
+/--
+Iterators for ranges implementing `RangeSize` support the `size` function.
+-/
+instance [Rxo.HasSize α] [UpwardEnumerable α] [LT α] [DecidableLT α] :
+    IteratorSize (Rxo.Iterator α) Id where
+  size it := match it.internalState.next with
+    | none => pure (.up 0)
+    | some next => pure (.up (Rxo.HasSize.size next it.internalState.upperBound))
+
+/--
+Returns the number of elements contained in the given range, given that ranges of the given
+type and shape support this function.
+-/
+@[always_inline, inline]
+def size [UpwardEnumerable α] [Least? α] [LT α] [DecidableLT α] (r : Rio α)
+    [IteratorSize (Rxo.Iterator α) Id] : Nat :=
+  Internal.iter r |>.size
+
+section Iterator
+
+theorem Internal.isPlausibleIndirectOutput_iter_iff
+    [UpwardEnumerable α] [LT α] [DecidableLT α] [Least? α]
+    [LawfulUpwardEnumerable α] [LawfulUpwardEnumerableLT α]
+    [LawfulUpwardEnumerableLeast? α] {r : Rio α} {a : α} :
+    (Internal.iter r).IsPlausibleIndirectOutput a ↔ a ∈ r := by
+  rw [Rxo.Iterator.isPlausibleIndirectOutput_iff]
+  constructor
+  · rintro ⟨n, hn, hu⟩
+    simp only [Membership.mem, LawfulUpwardEnumerableLT.lt_iff]
+    cases hr : (Internal.iter r).internalState.next
+    · simp [hr] at hn
+    · simpa [LawfulUpwardEnumerableLT.lt_iff] using hu
+  · intro hu
+    obtain ⟨init, hi, hia⟩ := LawfulUpwardEnumerableLeast?.least?_le a
+    simpa [iter, hi] using ⟨hia, hu⟩
+
+@[no_expose]
+instance {m} [UpwardEnumerable α]
+    [LT α] [DecidableLT α] [Least? α]
+    [LawfulUpwardEnumerable α] [LawfulUpwardEnumerableLT α]
+    [LawfulUpwardEnumerableLeast? α]
+    [Monad m] [Finite (Rxo.Iterator α) Id] :
+    ForIn' m (Rio α) α inferInstance where
+  forIn' r init f := by
+    haveI := Iter.instForIn' (α := Rxo.Iterator α) (β := α) (n := m)
+    refine ForIn'.forIn' (α := α) (Internal.iter r) init (fun a ha acc => f a ?_ acc)
+    simp only [Membership.mem] at ha
+    rwa [Internal.isPlausibleIndirectOutput_iter_iff] at ha
+
+end Iterator
+
+end Rio
+
+namespace Rii
+
+variable {α : Type u}
+
+/--
+Internal function that constructs an iterator for a `PRange`. This is an internal function.
+Use `PRange.iter` instead, which requires importing `Std.Data.Iterators`.
+-/
+@[always_inline, inline]
+def Internal.iter [UpwardEnumerable α] [Least? α] (_ : Rii α) : Iter (α := Rxi.Iterator α) α :=
+  ⟨⟨Least?.least?⟩⟩
+
+/--
+Returns the elements of the given range as a list in ascending order, given that ranges of the given
+type and shape support this function and the range is finite.
+-/
+@[always_inline, inline, expose]
+def toList [UpwardEnumerable α] [Least? α] (r : Rii α)
+    [Iterator (Rxi.Iterator α) Id α] [Finite (Rxi.Iterator α) Id]
+    [IteratorCollect (Rxi.Iterator α) Id Id] : List α :=
+  Internal.iter r |>.toList
+
+/--
+Returns the elements of the given range as an array in ascending order, given that ranges of the
+given type and shape are finite and support this function.
+-/
+@[always_inline, inline, expose]
+def toArray {α} [UpwardEnumerable α] [Least? α] (r : Rii α)
+    [Iterator (Rxi.Iterator α) Id α] [Finite (Rxi.Iterator α) Id]
+    [IteratorCollect (Rxi.Iterator α) Id Id] : Array α :=
+  Internal.iter r |>.toArray
+
+/--
+Iterators for ranges implementing `RangeSize` support the `size` function.
+-/
+instance [Rxi.HasSize α] [UpwardEnumerable α] :
+    IteratorSize (Rxi.Iterator α) Id where
+  size it := match it.internalState.next with
+    | none => pure (.up 0)
+    | some next => pure (.up (Rxi.HasSize.size next))
+
+/--
+Returns the number of elements contained in the given range, given that ranges of the given
+type and shape support this function.
+-/
+@[always_inline, inline]
+def size [UpwardEnumerable α] [Least? α] (r : Rii α) [IteratorSize (Rxi.Iterator α) Id] : Nat :=
+  Internal.iter r |>.size
+
+section Iterator
+
+theorem Internal.isPlausibleIndirectOutput_iter_iff
+    [UpwardEnumerable α] [Least? α] [LawfulUpwardEnumerable α] [LawfulUpwardEnumerableLeast? α]
+    {r : Rii α} {a : α} : (Internal.iter r).IsPlausibleIndirectOutput a ↔ a ∈ r := by
+  rw [Rxi.Iterator.isPlausibleIndirectOutput_iff]
+  constructor
+  · simp [Membership.mem]
+  · obtain ⟨init, hi, hia⟩ := LawfulUpwardEnumerableLeast?.least?_le a
+    simpa [Membership.mem, iter, hi] using hia
+
+@[no_expose]
+instance {m} [UpwardEnumerable α] [Least? α]
+    [LawfulUpwardEnumerable α] [LawfulUpwardEnumerableLeast? α]
+    [Monad m] [Finite (Rxi.Iterator α) Id] :
+    ForIn' m (Rii α) α inferInstance where
+  forIn' r init f := by
+    haveI := Iter.instForIn' (α := Rxi.Iterator α) (β := α) (n := m)
+    refine ForIn'.forIn' (α := α) (Internal.iter r) init (fun a ha acc => f a ?_ acc)
+    simp only [Membership.mem] at ha
+    rwa [Internal.isPlausibleIndirectOutput_iter_iff] at ha
+
+end Iterator
+
+end Rii
+
+end Std
